A bit more work on the "only need to run a finite number of steps" idea

TwoWayAutomata/Kozen/Execute.lean
@@ -1,7 +1,4 @@
 import Mathlib.Data.Fintype.Defs
-import Mathlib.Data.Fintype.Pigeonhole
-import Mathlib.Data.List.Basic
-import Mathlib.Data.List.Dedup
 
 import TwoWayAutomata.Kozen.Basics
 import TwoWayAutomata.Kozen.Configurations
@@ -9,79 +6,6 @@ import TwoWayAutomata.Kozen.Language
 import TwoWayAutomata.Kozen.Lemmas
 import TwoWayAutomata.Kozen.Movement
 import TwoWayAutomata.Kozen.Word
-
-lemma List.Chain.append_singleton {α : Type _} {R : α → α → Prop} {l : List α} {a b : α}
-  (hc : List.Chain R a l) (hr : R ((a :: l).getLast <| by simp) b) :
-    List.Chain R a (l ++ [b]) := by
-  induction hc with
-  | nil => simpa
-  | cons hr' hc ih =>
-    have := ih <| by simpa using hr
-    exact .cons hr' this
-
-lemma List.Chain.trim_singleton {α : Type _} {R : α → α → Prop} {l : List α} {a b : α}
-  (h : List.Chain R a (l ++ [b])) :
-    List.Chain R a l ∧ R ((a :: l).getLast <| by simp) b := by
-  induction l generalizing a with
-  | nil => simpa using h
-  | cons _ _ ih =>
-    simp only [cons_append, chain_cons] at h
-    simp [ih h.right, h]
-
-lemma List.Chain.get_step {α : Type _} {R : α → α → Prop} {a : α} {b : List α} (c : Chain R a b) (idx : Nat) (hidx : idx < b.length) :
-    have : idx < (a::b).length := Nat.lt_add_one_of_lt hidx; R (a :: b)[idx] b[idx] := by
-  cases c with
-  | nil => simp at hidx  -- Contradiction, idx < 0
-  | cons ha c' =>
-    cases idx with
-    | zero => exact ha
-    | succ idx' => apply c'.get_step idx'
-
-theorem List.pidgeon_hole {α : Type _} [DecidableEq α] [fin : Fintype α] (l : List α) (h : fin.card < l.length) : ∃ x : α, l.Duplicate x := by
-  obtain ⟨x, y, hne, hidx⟩ := Fintype.exists_ne_map_eq_of_card_lt (l.get) <| by simp [h]
-  use l.get x
-  rw [duplicate_iff_sublist]
-  if hord : x < y
-    then
-      suffices [l.get x, l.get y].Sublist l by rwa [←hidx] at this
-      have left : [l[x]].Sublist (l.take (x+1)) := by
-        rw [singleton_sublist, mem_take_iff_getElem]
-        suffices x.val < min (x.val+1) l.length by exists x, this
-        simp [x.is_lt]
-      have right : [l[y]].Sublist (l.drop (x+1)) := by
-        rw [singleton_sublist, mem_drop_iff_getElem]
-        have : y.val - (x.val + 1) + (x.val + 1) = y.val := by
-          rwa [Nat.sub_add_cancel]
-        use y.val - (x.val + 1), by rw [this]; exact y.is_lt
-        conv in _ + _ + _ =>
-          rw [Nat.add_comm, this]
-        simp
-      have : [l.get x, l.get y] = [l.get x] ++ [l.get y] := by simp
-      rw [this, append_sublist_iff]
-      use l.take (x+1), l.drop (x+1)
-      simp only [take_append_drop, get_eq_getElem, true_and]
-      exact ⟨left, right⟩
-    else
-      have : y < x := by simpa [hord] using Fin.lt_or_lt_of_ne hne
-      suffices [l.get y, l.get x].Sublist l by rwa [←hidx] at this
-      have left : [l[y]].Sublist (l.take (y+1)) := by
-        rw [singleton_sublist, mem_take_iff_getElem]
-        suffices y.val < min (y.val+1) l.length by exists y, this
-        simp [y.is_lt]
-      have right : [l[x]].Sublist (l.drop (y+1)) := by
-        rw [singleton_sublist, mem_drop_iff_getElem]
-        have : x.val - (y.val + 1) + (y.val + 1) = x.val := by
-          rwa [Nat.sub_add_cancel]
-        use x.val - (y.val + 1), by rw [this]; exact x.is_lt
-        conv in _ + _ + _ =>
-          rw [Nat.add_comm, this]
-        simp
-      have : [l.get y, l.get x] = [l.get y] ++ [l.get x] := by simp
-      rw [this, append_sublist_iff]
-      use l.take (y+1), l.drop (y+1)
-      simp only [take_append_drop, get_eq_getElem, true_and]
-      exact ⟨left, right⟩
-
 
 inductive RunResult : Type
   | accept : RunResult
@@ -92,325 +16,8 @@ namespace TwoDFA
 
 variable {α σ : Type*} {n : Nat} (m : TwoDFA α σ) (w : Word α n) 
 
-def stepTimes (steps : Nat) (strt : Config σ n) : Config σ n :=
-  match steps with
-  | 0 => strt
-  | k + 1 => m.stepConfig w <| stepTimes k strt
-
-theorem stepTimes_comm (steps : Nat) (strt : Config σ n) :
-    m.stepConfig w (m.stepTimes w steps strt) = m.stepTimes w steps (m.stepConfig w strt) := by
-  induction steps with
-  | zero => simp [stepTimes]
-  | succ k ih => simp [stepTimes, ih]
-
-theorem GoesTo_of_stepTimes {steps : Nat} {strt stp : Config σ n} (h : m.stepTimes w steps strt = stp) : m.GoesTo w strt stp := by
-  cases steps with
-  | zero =>
-    simp [stepTimes] at h
-    rw [h]
-  | succ k =>
-    rw [stepTimes, stepConfig_gives_nextConfig] at h
-    apply GoesTo.tail
-    · exact GoesTo_of_stepTimes (stp := m.stepTimes w k strt) rfl
-    · exact h
-
-@[ext]
-structure ExecTrace : Type _ where
-  strt : Config σ n
-  rest : List (Config σ n)
-  prf : rest.Chain (m.nextConfig w) strt
-
-namespace ExecTrace
-
-variable {m : TwoDFA α σ} {w : Word α n} 
-
-@[simp]
-def nil (cfg : Config σ n) : m.ExecTrace w where
-  strt := cfg
-  rest := []
-  prf := .nil
-
-@[simp]
-def cons (head : Config σ n) (tail : m.ExecTrace w) (h : m.nextConfig w head tail.strt) : m.ExecTrace w where
-  strt := head
-  rest := tail.strt :: tail.rest
-  prf := .cons h tail.prf
-
-def toList (trace : m.ExecTrace w) : List (Config σ n) :=
-  trace.strt :: trace.rest
-
-def lastCfg (trace : m.ExecTrace w) : Config σ n := 
-  match trace.rest with
-  | [] => trace.strt
-  | h :: t => (h :: t).getLast <| by simp
-
-theorem lastCfg_eq_toList_getLast {trace : m.ExecTrace w} : trace.lastCfg = trace.toList.getLast (by simp [toList]) := by
-  if h : trace.rest = []
-    then
-      conv =>
-        lhs
-        simp [lastCfg, h]
-      simp [toList, h]
-    else
-      have : trace.rest = trace.rest.head h :: trace.rest.tail := by simp
-      conv =>
-        lhs
-        unfold lastCfg
-        rw [this]
-        simp
-      simp [toList, h]
-
-def trans (t1 t2 : m.ExecTrace w) (h : m.nextConfig w t1.lastCfg t2.strt) : m.ExecTrace w where
-  strt := t1.strt
-  rest := t1.rest ++ t2.toList
-  prf := by
-    unfold toList
-    rw [List.chain_split]
-    refine ⟨?_, t2.prf⟩
-    apply List.Chain.append_singleton
-    · exact t1.prf
-    · rwa [lastCfg_eq_toList_getLast] at h
-
-def length (trace : m.ExecTrace w) : Nat := trace.rest.length + 1
-
-@[simp]
-theorem length_ne_0 (trace : m.ExecTrace w) : trace.length ≠ 0 := by simp [length]
-
-instance {trace : m.ExecTrace w} : NeZero trace.length where
-  out := trace.length_ne_0
-
-def get (trace : m.ExecTrace w) (idx : Fin (trace.length)) : Config σ n :=
-  trace.toList.get idx
-
-def split (trace : m.ExecTrace w) (idx : Fin (trace.length)) (h : idx ≠ ⟨0, by simp [length]⟩) : m.ExecTrace w × m.ExecTrace w :=
-  have h' : idx.val ≠ 0 := Fin.val_ne_of_ne h
-  have : trace.rest = (trace.rest.take <| idx.pred h) ++ trace.get idx :: trace.rest.drop idx := by
-    have valid : idx.val - 1 < trace.rest.length := by
-      rw [←Nat.add_one_lt_add_one_iff, Nat.sub_one_add_one h']
-      exact idx.is_lt
-    have : trace.rest[idx.val - 1]'valid :: List.drop (idx.val) trace.rest = List.drop (idx.val - 1) trace.rest := by
-      conv in List.drop _ _ => rw [←Nat.sub_one_add_one h']
-      apply List.getElem_cons_drop
-    simp [get, toList, List.getElem_cons, h', this]
-  have : List.Chain (m.nextConfig w) trace.strt (_ ++ [_]) ∧ List.Chain (m.nextConfig w) _ _ := by
-    rw [←List.chain_split, ←this]
-    exact trace.prf
-  ⟨⟨
-    trace.strt,
-    trace.rest.take <| idx.pred h,
-    List.Chain.trim_singleton this.left |>.left,
-  ⟩, ⟨
-    trace.get idx,
-    trace.rest.drop idx,
-    this.right,
-  ⟩⟩
-
-lemma split_left_lastCfg (trace : m.ExecTrace w) (idx : Fin (trace.length)) (h : idx ≠ 0) :
-    (trace.split idx h).1.lastCfg = trace.get (idx - 1) := by
-  simp [split, lastCfg, get]
-  cases hidx : idx.val - 1 with
-  | zero =>
-    have : (idx - 1).val = 0 := by rwa [Fin.val_sub_one_of_ne_zero h]
-    conv in _[_] => lhs; rw [this]
-    simp [toList]
-  | succ k =>
-    have : (idx - 1).val = k + 1 := by rwa [Fin.val_sub_one_of_ne_zero h]
-    conv in _[_] => lhs; rw [this]
-    simp only [toList, List.getElem_cons_succ]
-    cases htake : trace.rest.take (k+1) with
-    | nil =>
-      conv at htake =>
-        rw [List.take_eq_nil_iff]
-        simp only [Nat.add_eq_zero, one_ne_zero, and_false, false_or]
-      have len_one : trace.length = 1 := by simpa [length]
-      have := idx.is_lt
-      conv at this => rhs; rw [len_one]
-      rw [Nat.lt_one_iff] at this
-      rw [Fin.ne_iff_vne] at h
-      contradiction
-    | cons hd tl =>
-      simp only
-      conv in _ :: _ => rw [←htake]
-      rw [List.getLast_take]
-      suffices k < trace.rest.length by simp [List.getElem?_eq_getElem this]
-      have := idx.is_lt.trans' <| Nat.sub_one_lt <| Fin.val_ne_of_ne h
-      simpa [hidx, length]
-
-lemma split_connect (trace : m.ExecTrace w) (idx : Fin (trace.length)) (h : idx ≠ 0) : 
-    let (left, right) := trace.split idx h; m.nextConfig w left.lastCfg right.strt := by
-  split 
-  have h' : idx.val ≠ 0 := by simpa using Fin.val_ne_of_ne h
-  have hlen : trace.length ≠ 1 := by
-    by_contra hlen
-    have := idx.is_lt
-    conv at this => rhs; rw [hlen]
-    rw [Nat.lt_one_iff] at this
-    contradiction
-  next _ left right heq =>
-    conv at heq =>
-      simp [split]
-    rw [←heq.left, ←heq.right]
-    simp only [lastCfg]
-    rcases hrest : trace.rest.take (idx.val - 1) with _ | ⟨hd, tl⟩
-    · simp only
-      rcases List.take_eq_nil_iff.mp hrest with idx_one | rest_nil
-      -- trace.rest.take _ = []  ∧  ↑idx-1 = 0
-      · have one_mod_len : 1 % trace.toList.length = 1 := by rwa [Nat.one_mod_eq_one]
-        have idx_one : idx = 1 := by
-          rw [←Nat.add_one_inj, Nat.sub_one_add_one h', zero_add] at idx_one
-          rw [←Fin.val_inj, idx_one]
-          symm
-          simpa only [Fin.coe_ofNat_eq_mod, length, toList] using one_mod_len
-        rw [idx_one]
-        simp only [get, List.get_eq_getElem, Fin.coe_ofNat_eq_mod, one_mod_len]
-        simp [toList]
-        apply trace.prf.get_step 0
-      -- trace.rest.take _ = []  ∧  ↑idx-1 ≠ 0
-      · have := idx.is_lt
-        conv at this =>
-          simp only [length, rest_nil]
-          simp
-        contradiction
-    -- trace.rest.take _ = hd :: tl
-    · simp only
-      have _ : idx.val - 1 < trace.rest.length := by
-        have := idx.is_lt
-        unfold length at this
-        rwa [←Nat.add_one_lt_add_one_iff, Nat.sub_one_add_one h']
-      have hstep := trace.prf.get_step (idx.val - 1) <| by assumption
-      have _ : idx.val - 1 < (trace.strt :: trace.rest).length := by
-        simp only [List.length_cons]
-        apply Nat.lt_of_le_of_lt (m := idx.val)
-        · simp
-        · exact idx.is_lt
-      suffices (trace.strt :: trace.rest)[idx.val - 1] = (trace.rest.take (idx.val - 1)).getLast (by simp [hrest]) by
-        conv in hd :: tl => rw [←hrest]
-        rw [←this]
-        have : trace.get idx = trace.rest[idx.val-1] := by simp [get, toList, List.getElem_cons, h]
-        rwa [this]
-      have idx_ne_one : idx.val - 1 ≠ 0 := by
-        by_contra idx_one
-        simp [idx_one] at hrest
-      have := List.getLast_take (i := idx.val - 1) (l := trace.rest) <| by simp [hrest]
-      rw [this]
-      have : idx.val - 1 - 1 < trace.rest.length := by
-        apply Nat.lt_of_le_of_lt (m := idx.val - 1)
-        · simp
-        · assumption
-      have := List.getElem?_eq_getElem this
-      simp [this, List.getElem_cons, idx_ne_one]
-
-theorem split_trans (trace : m.ExecTrace w) (idx : Fin (trace.length)) (h : idx ≠ ⟨0, by simp [length]⟩) : 
-    (trace.split idx h).1.trans (trace.split idx h).2 (by have := trace.split_connect idx h; simpa) = trace := by
-  simp only [split, trans]
-  ext : 1
-  · rfl
-  · suffices trace.get idx :: trace.rest.drop idx.val = trace.rest.drop (idx.val - 1) by simp [toList, this]
-    have h' : idx.val ≠ 0 := by simpa using h
-    have : idx.val = idx.val - 1 + 1 := Nat.sub_one_add_one h' |>.symm
-    conv in List.drop _ _ => lhs; rw [this]
-    have : idx.val - 1 < trace.rest.length := by
-      have := idx.is_lt
-      unfold length at this
-      rwa [←Nat.add_one_lt_add_one_iff, Nat.sub_one_add_one h']
-    simp [get, toList, List.getElem_cons, h', this]
-
-end ExecTrace
-
-def traceSteps' (strt : Config σ n) : Nat → List (Config σ n)
-  | 0 => [strt]
-  | k + 1 => strt :: traceSteps' (m.stepConfig w strt) k
-
-lemma traceSteps'_nonempty (strt : Config σ n) (steps : Nat) : m.traceSteps' w strt steps ≠ [] := by
-  cases steps <;> simp [traceSteps']
-
-lemma traceSteps'_head (strt : Config σ n) : ∀ steps, ∃ l, m.traceSteps' w strt steps = strt :: l
-  | 0 => by use []; simp [traceSteps']
-  | k + 1 => by
-    use m.traceSteps' w (m.stepConfig w strt) k
-    simp [traceSteps']
-
-lemma traceSteps'_chain (steps : Nat) {strt head : Config σ n} {tail : List (Config σ n)} (htrace : m.traceSteps' w strt steps = head :: tail) :
-    tail.Chain (m.nextConfig w) head := by
-  cases steps with
-  | zero =>
-    -- Contradiction at htrace : m.traceSteps' w strt 0 = head :: h :: t
-    have : m.traceSteps' w strt 0 = [strt] := by simp [traceSteps']
-    simp [this] at htrace
-    rw [htrace.right]
-    exact .nil
-  | succ k =>
-    simp [traceSteps'] at htrace
-    cases tail with
-    | nil => simp [traceSteps'_nonempty, htrace.right]
-    | cons h t =>
-      apply List.Chain.cons
-      · rw [←stepConfig_gives_nextConfig, ←htrace.left]
-        obtain ⟨_, hhead⟩ := m.traceSteps'_head w (m.stepConfig w strt) k
-        simp [htrace.right] at hhead
-        exact hhead.left.symm
-      · exact traceSteps'_chain k htrace.right
-
-theorem traceSteps'_succ (steps : Nat) (strt : Config σ n) : m.traceSteps' w strt steps = (m.traceSteps' w strt (steps + 1)).dropLast := by
-  induction steps generalizing strt with
-  | zero => simp [traceSteps']
-  | succ k ih => 
-    unfold traceSteps'
-    suffices m.traceSteps' w (m.stepConfig w strt) (k + 1) =
-            (m.stepConfig w strt) :: m.traceSteps' w (m.stepConfig w <| m.stepConfig w strt) k by simp [ih, this]
-    conv => lhs; unfold traceSteps'; simp only
-
-def traceSteps (steps : Nat) (strt : Config σ n) : m.ExecTrace w :=
-  match h : m.traceSteps' w strt steps with
-  | [] => by have := m.traceSteps'_nonempty w strt steps; contradiction
-  | [single] => .nil single
-  | head :: tail => ⟨head, tail, traceSteps'_chain m w steps h⟩
-
-theorem traceSteps_length (steps : Nat) (strt : Config σ n) : (m.traceSteps w steps strt).length = steps + 1 := by
-  simp only [traceSteps]
-  split
-  case h_1 heq =>
-    have := m.traceSteps'_nonempty w strt steps
-    contradiction
-  case h_2 single heq =>
-    cases steps with
-    | zero => simp [ExecTrace.length]
-    | succ k =>
-      conv at heq =>
-        simp [traceSteps', traceSteps'_nonempty]
-      contradiction
-  case h_3 head tail tailne heq =>
-    simp only [ExecTrace.length]
-    induction steps generalizing tail with
-    | zero =>
-      simp [traceSteps'] at heq
-      simpa using heq.right
-    | succ k ih =>
-      have := m.traceSteps'_succ w k strt
-      rw [heq] at this
-      sorry
-
-theorem traceSteps'_getLast_eq_stepTimes (steps : Nat) (strt : Config σ n) :
-    m.stepTimes w steps strt = (m.traceSteps' w strt steps).getLast (traceSteps'_nonempty _ _ _ _) := by
-  match steps with
-  | 0 => simp [stepTimes, traceSteps']
-  | k+1 =>
-    simp only [stepTimes, traceSteps', List.getLast_cons <| traceSteps'_nonempty _ _ _ _]
-    have hind := traceSteps'_getLast_eq_stepTimes k <| m.stepConfig w strt
-    rwa [stepTimes_comm]
-
-theorem traceSteps_last_cfg_eq_traceSteps'_getLast (steps : Nat) (strt : Config σ n) :
-    (m.traceSteps w steps strt).lastCfg = (m.traceSteps' w strt steps).getLast (traceSteps'_nonempty _ _ _ _) := by
-  rcases steps with _zero | _one | _more
-  <;> simp [traceSteps, traceSteps', ExecTrace.lastCfg]
-
-theorem traceSteps_equiv_stepTimes (steps : Nat) (strt : Config σ n) : m.stepTimes w steps strt = (m.traceSteps w steps strt).lastCfg := by
-  trans
-  · exact m.traceSteps'_getLast_eq_stepTimes w steps strt
-  · symm; exact m.traceSteps_last_cfg_eq_traceSteps'_getLast w steps strt
-
 def execute [DecidableEq σ] [fin_cfgs : Fintype (Config σ n)] : RunResult :=
-  let last_config := m.stepTimes w fin_cfgs.card m.init
+  let last_config := m.runOn w fin_cfgs.card
   if last_config.state = m.accept
     then .accept
     else if last_config.state = m.reject
@@ -418,45 +25,59 @@ def execute [DecidableEq σ] [fin_cfgs : Fintype (Config σ n)] : RunResult :=
       -- We step as many times as there are unique configurations; if we haven't terminated yet we never will
       else .cycle
 
-theorem execute_accept_iff_stepTimes_state_eq_accept [DecidableEq σ] [fin_cfgs : Fintype (Config σ n)] :
-    m.execute w = .accept ↔ (m.stepTimes w fin_cfgs.card m.init).state = m.accept where
+theorem execute_accept_iff_runOn_state_eq_accept [DecidableEq σ] [fin_cfgs : Fintype (Config σ n)] :
+    m.execute w = .accept ↔ (m.runOn w fin_cfgs.card).state = m.accept where
   mp := by
     intro hexec
     by_contra hne
     simp [execute, hne] at hexec
-    if h : (m.stepTimes w (Fintype.card (Config σ n)) m.init).state = m.reject
+    if h : (m.runOn w (Fintype.card (Config σ n))).state = m.reject
       then simp [h] at hexec
       else simp [h] at hexec
   mpr := by
     intro heq
     simp [execute, heq]
 
-theorem execute_accept_iff_traceSteps_state_eq_accept [DecidableEq σ] [fin_cfgs : Fintype (Config σ n)] :
-    m.execute w = .accept ↔ (m.traceSteps w fin_cfgs.card m.init).lastCfg.state = m.accept := by
-  rw [execute_accept_iff_stepTimes_state_eq_accept, traceSteps_equiv_stepTimes]
-
-theorem duplicate_of_gt_maxSteps [DecidableEq σ] [fin_cfgs : Fintype (Config σ n)] (steps : Nat) (hstep : fin_cfgs.card < steps) :
-    ∃ c, (m.traceSteps w steps m.init).toList.Duplicate c := by
-  apply List.pidgeon_hole
+-- If steps > card, the same config must appear earlier in the run, and we can repeat that logic until we get steps' ≤ card
+theorem runOn_max_steps [Fintype σ] (steps : Nat) (cfg : Config σ n) (h : m.runOn w steps = cfg) :
+    ∃ steps' ≤ Fintype.card (Config σ n), m.runOn w steps' = cfg := by
   sorry
 
-theorem duplicate_of_not_accept_maxSteps [DecidableEq σ] [fin_cfgs : Fintype (Config σ n)]
-  (ha : (m.traceSteps w fin_cfgs.card m.init).lastCfg.state ≠ m.accept) (hr : (m.traceSteps w fin_cfgs.card m.init).lastCfg.state ≠ m.reject) :
-    ∃ c, (m.traceSteps w fin_cfgs.card m.init).toList.Duplicate c := by
-  sorry
-
-theorem todo [DecidableEq σ] [fin_cfgs : Fintype (Config σ n)] {steps : Nat} {strt : Config σ n} (h : fin_cfgs.card < steps) :
-    (m.traceSteps w steps strt).lastCfg.state = m.accept ↔ (m.traceSteps w fin_cfgs.card strt).lastCfg.state = m.accept := by
-  sorry
+theorem accepts_iff_runOn_max_eq_accept [Fintype σ] : m.accepts w ↔ ∃ i, m.runOn w (Fintype.card (Config σ n)) = ⟨m.accept, i⟩ where
+  mp := by
+    rintro ⟨pos, hreach⟩
+    obtain ⟨steps, hrun⟩ := runOn_of_reaches (h := hreach)
+    rcases em (steps ≤ Fintype.card (Config σ n)) with hsteps | _
+    case' inr =>
+      -- In the steps > card case, we use runOn_max_steps to get an early-enough point in the run that is the same configuration
+      obtain ⟨steps, hsteps, hrun⟩ := runOn_max_steps (h := hrun)
+    all_goals
+      clear * - hsteps hrun
+      let remaining := Fintype.card (Config σ n) - steps
+      have : steps + remaining = Fintype.card (Config σ n) := by simp [remaining, hsteps]
+      rw [←this]; clear this
+      use (m.runOn w (steps + remaining)).idx
+      ext : 1 <;> simp only
+      apply m.accept_preserve_state w pos (m.runOn w (steps + remaining))
+      rw [←hrun]
+      apply runOn_GoesTo
+  mpr := by
+    rintro ⟨i, hrun⟩
+    use i
+    rw [←hrun]
+    apply reaches_runOn
 
 theorem accepts_iff_execute_eq_accept [DecidableEq σ] [Fintype σ] : m.accepts w ↔ m.execute w = .accept := by
-  rw [execute_accept_iff_traceSteps_state_eq_accept]
+  rw [execute_accept_iff_runOn_state_eq_accept, accepts_iff_runOn_max_eq_accept]
   constructor
   -- m.accepts w → m.execute w = .accept
-  · intro h
-    sorry
+  · rintro ⟨_, hrun⟩
+    rw [hrun]
   -- m.execute w = .accept → m.accepts w
   · intro h
-    sorry
+    use (m.runOn w (Fintype.card (Config σ n))).idx
+    ext : 1
+    · exact h
+    · rfl
 
 end TwoDFA
